heap/down/path1_verif.v
@@ -4,6 +4,7 @@ Require Import heap.program.
 Require Import heap.definitions.
 Require Import heap.annotation.
 Require heap.down.path1.
+Require Import SetsClass.SetsClass.
 
 Module SH_Proof <: STRAIGHTLINE_HOARE_TRIPLE_PROOF.
 
@@ -21,7 +22,7 @@ Proof.
   Intros.
   forward.
   forward.
-  assert ((Int.shl (IntRepr pos1) (IntRepr 1)) = Int.repr (pos1 * 2)). {
+  assert ((Int.shl (IntRepr pos1) (IntRepr 1)) = Int.repr (2 * pos1)). {
     unfold Int.shl.
     unfold Z.shiftl.
     simpl.
@@ -29,19 +30,20 @@ Proof.
     f_equal; lia.
   }
   rewrite H3, Int.signed_repr in H1 by rep_lia.
-  assert (Int.unsigned (Int.shl (IntRepr pos1) (IntRepr 1)) = pos1 * 2). {
+  assert (Int.unsigned (Int.shl (IntRepr pos1) (IntRepr 1)) = 2 * pos1). {
     rewrite H3.
     rewrite Int.unsigned_repr by rep_lia.
     reflexivity.
   }
   forward.
+  rewrite H12.
   forward.
   forward.
   forward.
+  rewrite H3.
   forward.
-  rewrite H3 in H13.
   rewrite H3 in H14.
-  assert (Int.or (IntRepr (pos1 * 2)) (IntRepr 1) = IntRepr(pos1 * 2 + 1)). {
+  assert (Int.or (IntRepr (2 * pos1)) (IntRepr 1) = IntRepr(2 * pos1 + 1)). {
     unfold Int.or.
     f_equal.
     rewrite !Int.unsigned_repr by rep_lia.
@@ -49,36 +51,54 @@ Proof.
   }
   rewrite H15 in H14.
   rewrite Int.signed_repr in H14 by rep_lia.
-  assert (Int.unsigned (Int.or (Int.shl (IntRepr pos1) (IntRepr 1)) (IntRepr 1))  = pos1 * 2 + 1). {
+  assert (Int.unsigned (Int.or (Int.shl (IntRepr pos1) (IntRepr 1)) (IntRepr 1))  = 2 * pos1 + 1). {
     rewrite H3, H15.
     rewrite Int.unsigned_repr by rep_lia.
     reflexivity.
   }
   forward.
+  rewrite H16.
   forward.
   forward.
   forward.
+  rewrite H3, H15.
   forward.
-  forward_call (Znth (pos1 * 2 + 1) Hl0, Znth pos1 Hl0, 
-                field_address (tarray tint Maxsize) [ArraySubsc (pos1 * 2 + 1)] a0,
+  assert_PROP (field_compatible (tarray tint Maxsize) [] a0) by entailer!.
+  forward_call (Znth (2 * pos1 + 1) Hl0, Znth pos1 Hl0, 
+                field_address (tarray tint Maxsize) [ArraySubsc (2 * pos1 + 1)] a0,
                 field_address (tarray tint Maxsize) [ArraySubsc pos1] a0,
                 field_address (tarray tint Maxsize) [ArraySubsc pos1] a0,
-                field_address (tarray tint Maxsize) [ArraySubsc (pos1 * 2 + 1)] a0).
+                field_address (tarray tint Maxsize) [ArraySubsc (2 * pos1 + 1)] a0).
   {
     entailer!.
     split.
-    + f_equal.
-      apply offset_val_field_address; [lia | tauto].
-    + f_equal.
-      rewrite H3, H15, floyd.forward.sem_add_pi'.
-      - apply offset_val_field_address; [lia | tauto].
-      - tauto. 
-      - tauto.
-      - rep_lia. 
+    + f_equal; apply offset_val_field_address; [lia | tauto].
+    + f_equal; apply offset_val_field_address; [lia | tauto].
   }
   {
-     
+    sep_apply (int_array_with_two_holes a0 Hl0 Maxsize pos1 (2 * pos1 + 1));
+      [lia | lia | lia | entailer!].  
   }
+  forward.
+  Exists (list_swap Hl0 pos1 (2 * pos1 + 1)) (2 * pos1 + 1) a0 (Vint (IntRepr (2 * pos1 + 1))) (Vint (IntRepr size0)).
+  entailer!.
+  2: {
+    sep_apply (int_array_with_two_holes_inv a0 Hl0 pos1 (2 * pos1 + 1) (Znth (2 * pos1 + 1) Hl0) (Znth pos1 Hl0));
+      [lia | lia | entailer!].
+  }
+  split.
+  2: apply all_int_swap; [tauto | lia | lia].
+  unfold down_inv.
+  etransitivity_n1; [apply H | ].
+  rewrite !Int.signed_repr in H13, H17.
+  2: apply all_int_Znth; [tauto | lia].
+  2: apply all_int_Znth; [tauto | lia].
+  2: apply all_int_Znth; [tauto | lia].
+  2: apply all_int_Znth; [tauto | lia].
+  unfold list_relation.list_down_succeed.
+  right; left.
+  list_relation.try_list_unfold_witout_Z.
+  repeat split.
 Admitted.
 
 End SH_Proof.
